Source/DafnyCore/AST/Statements/Assignment/UpdateStmt.cs
@@ -81,7 +81,7 @@ public class UpdateStmt : ConcreteUpdateStatement, ICloneable<UpdateStmt>, ICanR
   /// errorCountBeforeCheckingLhs is passed in so that this method can determined if any resolution errors were found during
   /// LHS or RHS checking, because only if no errors were found is update.ResolvedStmt changed.
   /// </summary>
-  public void Resolve(ModuleResolver resolver, ResolutionContext resolutionContext) {
+  public override void Resolve(ModuleResolver resolver, ResolutionContext resolutionContext) {
     Contract.Requires(this != null);
     Contract.Requires(resolutionContext != null);
 
