Source/DafnyCore/Resolver/PreType/INewOrOldResolver.cs
@@ -16,4 +16,5 @@ public interface INewOrOldResolver {
   void CheckIsLvalue(Expression expression, ResolutionContext resolutionContext);
   void ConstrainTypeExprBool(Expression expression, string message);
   void ResolveStatement(Statement statement, ResolutionContext resolutionContext);
+  void ResolveTypeRhs(TypeRhs typeRhs, Statement statement, ResolutionContext resolutionContext);
 }
