Source/IntegrationTests/TestFiles/LitTests/LitTest/ast/assume.dfy
@@ -1,6 +1,6 @@
-// RUN: %testDafnyForEachResolver "%s"
+// RUN: %testDafnyForEachResolver "%s" -- --allow-axioms=false 
 // NONUNIFORM: warning will be the same for all back-end
-// RUN: ! %run --allow-axioms:false "%s" >> "%t"
+// RUN: ! %run --standard-libraries --allow-axioms:false "%s" > "%t"
 // RUN: %diff "%s.expect" "%t"
 
 method Foo() {
@@ -10,5 +10,43 @@ method Foo() {
  var xs := { 1, 2 };
  var x :| assume x in xs;
 
- var ys :- assume { 1 }; 
+ var ys :- assume Some(3); 
+}
+
+/** This datatype is the conventional Some/None datatype that is often used
+  in place of a reference or null.
+*/
+datatype Option<+T> = None | Some(value: T) {
+
+    /** True if is None */
+    predicate IsFailure() {
+      None?
+    }
+
+    /** Converts a None result to an Option value with a different value type. */
+    function PropagateFailure<U>(): Option<U>
+      requires None?
+    {
+      None
+    }
+
+    /** Returns the value encapsulated in Some */
+    function Extract(): T
+      requires Some?
+    {
+      value
+    }
+
+    /** Returns the value encapsulated in Some or a default value if None */
+    function GetOr(default: T): T {
+      match this
+      case Some(v) => v
+      case None() => default
+    }
+
+    /** Applies the given function to convert the Option to something else  */
+    function Map<FC>(rewrap: Option<T> -> FC): FC
+    {
+      rewrap(this)
+    }
 }
